\section{Basics}

Taylor: $f(a)+\tfrac{f'(a)}{1!}(x-a) + \tfrac{f''(a)}{2!}(x-a)^2 + ...$ \\
General p-norm: $\norm{ x }_p = (\sum_{i=1}^n |x_i|^p)^{1/p}$\\
Entropy: $H(X)=\E_X[-\log P(X)]$\\
KL diverg.: $D_\text{KL}(P \parallel Q) = \int_{x\in\mathcal{X}} P(x) \log\left(\frac{P(x)}{Q(x)}\right)$\\
Power series of exponential: $\exp(x) := \sum_{k = 0}^{\infty} \frac{x^k}{k!}$\\
Cauchy-Schwarz: $|\E[X,Y]|^2 \leq \E[X^2] \E[Y^2]$ 

\subsection*{Probability / Statistics}
Gaussian:
$f(x) = \frac{1}{\sqrt{2\pi \sigma^2}} e^{- \frac{1}{2} \frac{(x-\mu)^2}{\sigma^2}}, \mathcal{N}(x|\mu, \sigma)$\\
$f(x) = \frac{1}{\sqrt{(2\pi)^d\det\Sigma}} e^{- \frac{1}{2} (x-\mu)^T \Sigma^{-1} (x-\mu)}, \mathcal{N}(x|\mu, \Sigma)$\\
$\ln(p(x|\mu, \Sigma)) {=} {-}\tfrac{d}{2}\ln(2\pi) {-} \tfrac{\ln|\Sigma|}{2} {-} \tfrac{1}{2}(x{-}\mu)^T\Sigma(x{-}\mu)$ \\
$X {\sim} \mathcal{N}(\mu,\Sigma)$, $Y{=}A{+}BX \Rightarrow Y{\sim}\mathcal{N}(A{+}B\mu,B\Sigma B^T)$\\
Binomial: $f(k,n,p) {=} Pr(X=k) {=} \binom nk p^k (1{-}p)^{n{-}k}$\\
Beta: $p(x|a,b)=\frac{1}{B(a,b)}\cdot x^{a-1}(1-x)^{b-1}$, where: $a,b>0$ and $B(a,b)=\frac{\Gamma (a)\Gamma(b)}{\Gamma (a+b)}$, with: $\Gamma(a)=\int_0^\infty e^{-x}x^{a-1}dx$
% Condition number: $\kappa(A)=\frac{\sigma_{max}(A)}{\sigma_{min}(A)}$ \\

\subsection*{Jensen's inequality}
	X R.V. \& $f(X)$ convex: $f(\mathbb{E}[X]) \leq \mathbb{E}[f(X)]$

\subsection*{Moments}
\begin{inparaitem}[\color{red}\textbullet]
% Variance
\item $Var[X]=\int_x(x-\mu)^2p(x) dx$ \\
\item $Var[X]=E[(X-E[X])^2]=E[X^2]-E[X]^2$ \\
\item $Var[X{+}Y]=Var[X]{+}Var[Y]{+}2Cov[X,Y]$ \\
% Covariance
\item $Cov[X,Y] = E[(X - E[X])(Y - E[Y])] = E[XY] - E[X]E[Y]$ \\
% \item $K_{\bm{XY}} = cov(X,Y) = E[XY^T] - E[X]E[Y^T]$
\item $Cov[aX,bY]{=}abCov[X,Y]$
\end{inparaitem}

\subsection*{Calculus}
\begin{inparaitem}[\color{red}\textbullet]
	\item Part.: $\int u(x)v'(x) dx = u(x)v(x) - \int v(x)u'(x) dx$\\
	\item $|x|'=x/|x|$\\
% 	\item Chain r.: $\frac{f(y)}{g(x)} = \frac{dz}{dx} \Big|_{x=x_0}= \frac{dz}{dy}\Big|_{z=g(x_0)}\cdot \frac{dy}{dx} \Big|_{x=x_0}$ \\
	%\item $g_x(1) = g_x(0) + g'_x(0) + \int_{0}^{1} g_x''(s)(1-s) ds$ \\
	%\item $g(\mathbf{w}+\delta) - g(\mathbf{w}) = %\int_{\mathbf{w}}^{\mathbf{w+\delta}} \nabla g(\mathbf{u}) du = (\int_{0}^{1} \nabla g(\mathbf{w}+t\delta)dt) \cdot \delta$\\
	\item $\frac{\partial}{\partial \mathbf{x}}(\mathbf{b}^\top \mathbf{x}) = \frac{\partial}{\partial \mathbf{x}}(\mathbf{x}^\top \mathbf{b}) = \mathbf{b}$
	\item $\frac{\partial}{\partial \mathbf{x}}(\mathbf{x}^\top \mathbf{x}) = 2\mathbf{x}$ \\
	\item $\frac{\partial}{\partial \mathbf{x}}(\mathbf{x}^\top \mathbf{A}\mathbf{x}) = (\mathbf{A}^\top + \mathbf{A})\mathbf{x} \stackrel{\text{\tiny A sym.}}{=} 2\mathbf{A}\mathbf{x}$ \\
	\item $\frac{\partial}{\partial \mathbf{x}}(\mathbf{b}^\top \mathbf{A}\mathbf{x}) = \mathbf{A}^\top \mathbf{b}$
	\item $\frac{\partial}{\partial \mathbf{X}}(\mathbf{c}^\top \mathbf{X} \mathbf{b}) = \mathbf{c}\mathbf{b}^\top$ \\
	\item $\frac{\partial}{\partial \mathbf{X}}(\mathbf{c}^\top \mathbf{X}^\top \mathbf{b}) = \mathbf{b}\mathbf{c}^\top$
	\item $\frac{\partial}{\partial \mathbf{x}}(\| \mathbf{x}-\mathbf{b} \|_2) = \frac{\mathbf{x}-\mathbf{b}}{\|\mathbf{x}-\mathbf{b}\|_2}$ \\
	\item $\frac{\partial}{\partial \mathbf{x}}(\|\mathbf{x}\|^2_2) = \frac{\partial}{\partial \mathbf{x}} (\|\mathbf{x}^\top \mathbf{x}\|_2) = 2\mathbf{x}$\\
% 	\item $\frac{\partial}{\partial \mathbf{X}}(\|\mathbf{X}\|_F^2) = 2\mathbf{X}$ \\
	\item Trace trick: $x^T A x \stackrel{\text{\tiny inner product}}{=} Tr(x^T A x) \stackrel{\text{\tiny cyclic permut.}}{=} Tr(x x^T A) = Tr(A x x^T)$ \\
	\item $\tfrac{\partial}{\partial A} Tr(AB) {=} B^T$
	\item $\frac{\partial}{\partial A} log|A| {=} A^{-T}$ \\
	\item $\sigma(x) = \frac{1}{1+\exp(-x)} \Rightarrow \nabla \sigma(x)=\sigma(x)(1-\sigma(x) $ \\
% 	\item $\nabla \text{sigmoid}(x) = \text{sigmoid}(x)(1-\text{sigmoid}(x))$ \\
	\item $tanhx {=} \frac{sinhx}{coshx} {=} \frac{e^{x}-e^{-x}}{e^{x} + e^{x}}$
	\item $\nabla \text{tanh}(x) = 1-\text{tanh}^2(x)$ 

\end{inparaitem}
% \subsection*{Probability / Statistics}
% \begin{compactdesc}
% % 	\item[Bayes' Rule]$ P(Y|X) = \frac{P(X|Y)P(Y)}{P(X)}$\\
% % 	\item[MGF] $\mathbf{M}_X(t)=\mathbb{E}[e^{\mathbf{t}^T \mathbf{X}}]$, $\mathbf{X}=(X_1,.., X_n) $
% \end{compactdesc}

